theory/cadeque/vector.v
@@ -1,0 +1,44 @@
+From Coq Require Import Program List.
+Import ListNotations.
+From Equations Require Import Equations.
+
+(* A type for vectors. *)
+Inductive vector (A : Type) : nat -> Type :=
+| V0 {u : nat} : vector A u
+| V1 {u : nat} : A -> vector A (1 + u)
+| V2 {u : nat} : A -> A -> vector A (2 + u)
+| V3 {u : nat} : A -> A -> A -> vector A (3 + u)
+| V4 {u : nat} : A -> A -> A -> A -> vector A (4 + u)
+| V5 {u : nat} : A -> A -> A -> A -> A -> vector A (5 + u)
+| V6 {u : nat} : A -> A -> A -> A -> A -> A -> vector A (6 + u).
+Arguments V0 {A u}.
+Arguments V1 {A u}.
+Arguments V2 {A u}.
+Arguments V3 {A u}.
+Arguments V4 {A u}.
+Arguments V5 {A u}.
+Arguments V6 {A u}.
+
+Set Equations Transparent.
+
+(* Returns the sequence associated to a vector. *)
+Equations vector_seq {A u} : vector A u -> list A :=
+vector_seq V0 := [];
+vector_seq (V1 a) := [a];
+vector_seq (V2 a b) := [a] ++ [b];
+vector_seq (V3 a b c) := [a] ++ [b] ++ [c];
+vector_seq (V4 a b c d) := [a] ++ [b] ++ [c] ++ [d];
+vector_seq (V5 a b c d e) := [a] ++ [b] ++ [c] ++ [d] ++ [e];
+vector_seq (V6 a b c d e f) := [a] ++ [b] ++ [c] ++ [d] ++ [e] ++ [f].
+
+(* Returns the number of elements contained in a vector. *)
+Equations vector_size {A u} (v : vector A u) : nat :=
+vector_size V0 := 0;
+vector_size (V1 _) := 1;
+vector_size (V2 _ _) := 2;
+vector_size (V3 _ _ _) := 3;
+vector_size (V4 _ _ _ _) := 4;
+vector_size (V5 _ _ _ _ _) := 5;
+vector_size (V6 _ _ _ _ _ _) := 6.
+
+Unset Equations Transparent.
